QS.v
@@ -3,26 +3,33 @@ Import ListNotations.
 Require Import DFA.
 Local Open Scope Z_scope.
 
+(* Queueing Systems *)
+
 Module Type QS (dfa : DFA).
   Include DFAUtils dfa.
-  
-  Variable count_event : dfa.B -> Z.
-  Variable n0 : Z.
-  Variable n1 : Z.
-  Variable n : Z.
-  Axiom n_correct : n >= n0.
-  Axiom n1_correct : n1 <= n0.
+
+  Parameters
+    (count_event : dfa.B -> Z)
+      (* a function that describes the number of items added to the buffer by some given event *)
+    (init_items min_items max_items : Z)
+      (* the specified countings for the initial, minimum and maximum itens inside the buffer *)
+    (max_items_correct : max_items >= init_items)
+    (min_items_correct : min_items <= init_items)
+      (* min_items <= init_items <= max_items *)
+    .
 End QS.
 
 Module QSUtils (dfa : DFA).
 Include QS dfa.
 
+(* a function that counts the number of buffered items based on the past events *)
 Fixpoint count_buffer w :=
   match w with
   | e::w' => count_event e + count_buffer w'
   | nil => 0
   end.
 
+(* count_buffer is pseudo-distributive, meaning that we can count the events in any order. *)
 Lemma count_buffer_distr w1 w2 :
   count_buffer (w1 ++ w2) = count_buffer w1 + count_buffer w2.
 Proof.
@@ -31,12 +38,14 @@ Proof.
   simpl; rewrite IH; omega.
 Qed.
 
+(* for w1=w and w2=[e] *)
 Lemma count_buffer_distr' w e :
   count_buffer (w ++ [e]) = count_buffer w + (count_event e).
 Proof.
   rewrite count_buffer_distr; simpl; omega.
 Qed.
 
+(* the number of items added by w^n is equal to the number of items added by w multiplied by n. *)
 Theorem count_word_pow: forall w n,
   count_buffer (word_pow w n) = (Z.of_nat n) * (count_buffer w).
 Proof.
@@ -47,60 +56,59 @@ Proof.
   omega.
 Qed.
 
-Lemma q0_cycle: forall w n,
-  ixtransition w = (q0) -> ixtransition (word_pow w n) = (q0).
-Proof.
-  intros w n H.
-  induction n as [|n IH]. auto.
-  unfold ixtransition in *;
-  simpl;
-  rewrite xtransition_distr, H;
-  auto.
-Qed.
-
+(* a function that lists the sequences of events of a given list that transition into a given state *)
 Fixpoint gen_words q (l:list (list B)) :=
   match l with
-  | w::l' => if A_decidable (ixtransition w) q then w::gen_words q l' else gen_words q l'
+  | w::l' => if A_eq_dec (ixtransition w) q then w::gen_words q l' else gen_words q l'
   | nil => nil
   end.
 
-Lemma gen_words_correct1 q l : forall w,
-  l <> nil -> In w (gen_words q l) -> ixtransition w = q.
+(* Every sequence of events returned by gen_words must be correct. *)
+Lemma gen_words_correct q l : forall w,
+  In w (gen_words q l) -> ixtransition w = q.
 Proof.
-  intros w H H0.
+  intros w H0;
   induction l as [|w' l' IH].
   - contradiction.
   - destruct l' as [|w'' l'].
-    + simpl in H0; destruct (A_decidable (ixtransition w') q).
-      inversion H0. rewrite <- H1; auto. inversion H1. inversion H0.
-    + simpl in *. destruct (A_decidable (ixtransition w') q).
-      inversion H0. rewrite <- H1; auto.
-      apply IH. intro contra; discriminate. apply H1.
-      apply IH. intro contra; discriminate. auto.
+    + simpl in H0; destruct (A_eq_dec (ixtransition w') q).
+      inversion H0 as [H|H].
+      rewrite <- H; auto.
+      destruct H.
+      destruct H0.
+    + simpl in *. destruct (A_eq_dec (ixtransition w') q) as [H|H].
+      inversion H0 as [H1|H1].
+      rewrite <- H1; auto.
+      1,2: apply IH; auto.
 Qed.
 
-Lemma gen_words_correct q l : forall w,
+(* Every sequence of events in l that transitions into q is in gen_words q l. *)
+Lemma gen_words_complete q l : forall w,
   In w l -> ixtransition w = q -> In w (gen_words q l).
 Proof.
   intros w H H0.
   induction l as [|w' l' IH]; inversion H; simpl.
-  - destruct (A_decidable (ixtransition w') q) eqn:H2.
+  - destruct (A_eq_dec (ixtransition w') q) eqn:H2.
     + left; auto.
     + rewrite <- H1 in H0; contradiction.
-  - destruct (A_decidable (ixtransition w') q). right; apply IH; auto.
+  - destruct (A_eq_dec (ixtransition w') q). right; apply IH; auto.
     apply IH; auto.
 Qed.
 
+(* a function that lists the sequences of events of a given list that transition into a given state
+  and whose length is less or equal to a given number *)
 Definition all_gen_words_le q n := gen_words q (all_words_le n).
 
-Lemma all_gen_words_le_correct q n : forall w,
-  q <> (sink) -> ixtransition w = q -> (length w <= n)%nat ->
+(* Every generated sequence of events that transition into q and whose length is less or equal to n
+  is in all_gen_words_le q n. *)
+Lemma all_gen_words_le_generated q n : forall w,
+  q <> sink -> ixtransition w = q -> (length w <= n)%nat ->
   In w (all_gen_words_le q n).
 Proof.
   unfold all_gen_words_le;
   intros w H H0 H1;
-  apply gen_words_correct.
-  apply all_words_le_correct;
+  apply gen_words_complete.
+  apply all_words_le_generated;
   rewrite <- H0 in H.
   1-3: auto.
 Qed.
