QSUpperBound.v
@@ -7,63 +7,83 @@ Module QSUpperBound (dfa : DFA).
 
 Include QSUtils dfa.
 
-Definition n_upper_bounded := forall w, is_generated w -> n0 + count_buffer w <= n.
+(* the queueing system is upper bounded if all of its generated sequences of events respect the number
+  of maximum items in the buffer *)
+Definition upper_bounded := forall w, generates w -> init_items + count_buffer w <= max_items.
 
+(*
+  We can construct a function f that gives the maximum number of items in the buffer in a given state following
+ this constraints:
+  -> f applied to the initial state gives a number greater or equal to the number of initial items
+  -> for every tangible state q, f applied to every transition starting from q through e gives a number greater or
+    equal to f applied to q plus count_event e
+  --
+  We shall now prove that this constraints are correct.
+*)
+
+(* The number of items counted from a given generated sequence of events must be less or equal to f applied
+  to its extended transition. *)
 Lemma buffer_count_leq_f : forall f,
-    ( f (q0) >= (n0) /\ forall q, In q (Q) -> is_tangible q -> forall e, In e (E) ->
-        f (delta q e) >= f q + count_event e )
-    -> forall w, is_generated w -> n0 + count_buffer w <= f (ixtransition w).
+    ( f state0 >= (init_items) /\ forall q, In q states -> is_tangible q -> forall e, In e events ->
+        f (transition q e) >= f q + count_event e )
+    -> forall w, generates w -> init_items + count_buffer w <= f (ixtransition w).
 Proof.
   intros f [H H0] w H10;
   induction w as [|e w' IH] using @rev_ind.
   - unfold ixtransition; simpl; omega.
-  - pose H10 as H1; apply prefix_closed in H1; fold is_generated in H1; pose H1 as H2;
+  - pose H10 as H1; apply gen_prefix_closed in H1; fold generates in H1; pose H1 as H2;
       apply IH in H2.
     unfold ixtransition, count_buffer; rewrite ixtransition_distr, count_buffer_distr';
       fold ixtransition xtransition count_buffer.
-    unfold is_generated in H1; remember (ixtransition w') as q eqn:H3.
+    unfold generates in H1; remember (ixtransition w') as q eqn:H3.
     rewrite H3; simpl; rewrite <- H3.
-    remember (delta q e) as q' eqn:H4.
+    remember (transition q e) as q' eqn:H4.
     cut (f q' >= f q + count_event e).
     omega.
     rewrite H4.
-    assert (H5: delta q e <> sink).
-      unfold is_generated in H10; rewrite ixtransition_distr in H10;
+    assert (H5: transition q e <> sink).
+      unfold generates in H10; rewrite ixtransition_distr in H10;
       simpl in H10; rewrite <- H3 in H10; auto.
-    apply (delta_correct) in H5.
+    apply (transition_correct) in H5.
     apply H0.
     2: split; auto; eexists; fold ixtransition; symmetry; apply H3.
     1-2: intuition.
 Qed.
 
+(*
+  This lemma helps prove pumping_buffer.
+  Every pumping sequence w1 ++ w2^n ++ w3 is such that:
+  1 - count_buffer w2 <= 0 and count_buffer (w1 ++ w2^n ++ w3) <= count_buffer (w1 ++ w3)
+  2 - count_buffer w2 > 0 and the queueing system is not upper bounded
+*)
 Lemma pumping_buffer1 q : forall w,
-  n_upper_bounded -> ixtransition w = q -> q <> (sink) ->
-  (length w >= length (Q))%nat ->
+  upper_bounded -> ixtransition w = q -> q <> (sink) ->
+  (length w >= length states)%nat ->
   exists w', ixtransition w' = q /\ (length w' < length w)%nat /\
   count_buffer w' >= count_buffer w.
 Proof.
   intros w H H0 H1 H2;
-  assert (H10: exists m, Z.of_nat m >= n - n0 - count_buffer w + 1). {
-    assert (H3: 0 <= (n - n0 - count_buffer w + 1)).
-      unfold n_upper_bounded, is_generated in H; rewrite <- H0 in H1; apply H in H1; omega.
+  assert (H10: exists m, Z.of_nat m >= max_items - init_items - count_buffer w + 1). {
+    assert (H3: 0 <= (max_items - init_items - count_buffer w + 1)).
+      unfold upper_bounded, generates in H; rewrite <- H0 in H1; apply H in H1; omega.
     apply Z_of_nat_complete in H3; destruct H3 as [n1 H3];
     exists n1; omega.
   }
   destruct H10 as [m H10].
-  apply pumping_pow with (n:=S m) in H2;
-  destruct H2 as [w1 [w2 [w3 [H2 [H3 [H4 H6]]]]]];
+  apply pumping in H2;
+  destruct H2 as [w1 [w2 [w3 [H2 [H3 H4]]]]];
   fold ixtransition in H4;
   destruct (Z_le_gt_dec (count_buffer w2) 0) as [H5|H5].
   - exists (w1++w3); repeat split.
-    + rewrite <- H0; unfold ixtransition; auto.
+    + rewrite <- H0; unfold ixtransition; specialize (H4 0%nat);
+      simpl in H4; auto.
     + rewrite H2, app_length, app_length, app_length.
       assert (length w2 > 0)%nat.
         destruct w2; try contradiction; simpl; omega.
       omega.
-    + rewrite H2.
-      rewrite count_buffer_distr, count_buffer_distr, count_buffer_distr.
+    + rewrite H2, count_buffer_distr, count_buffer_distr, count_buffer_distr;
       omega.
-  - assert (contra: n0 + count_buffer (w1 ++ word_pow w2 (S m) ++ w3) > (n)). {
+  - assert (contra: init_items + count_buffer (w1 ++ word_pow w2 (S m) ++ w3) > max_items). {
       rewrite count_buffer_distr, count_buffer_distr;
       rewrite count_word_pow.
       replace (count_buffer w1 + (Z.of_nat (S m) * count_buffer w2 + count_buffer w3)) with
@@ -72,23 +92,25 @@ Proof.
       rewrite Nat2Z.inj_succ, <- Z.add_1_r, Z.mul_add_distr_r; omega.
       nia.
     }
-    assert (contra0: is_generated (w1 ++ word_pow w2 (S m) ++ w3)).
-      unfold is_generated; fold ixtransition; rewrite H4, H0;
+    assert (contra0: generates (w1 ++ word_pow w2 (S m) ++ w3)).
+      unfold generates; fold ixtransition; rewrite H4, H0;
       auto.
     apply H in contra0. omega.
 Qed.
 
+(* If the queueing system is upper bounded, for every generated sequence of events w with length greater or equal
+  to the number of states, exists a sequence of events that transition into ixtransition w and counts a number of
+  items greater or equal to count_buffer w. *)
 Lemma pumping_buffer q : forall w,
-  n_upper_bounded -> ixtransition w = q -> q <> (sink) ->
-  (length w >= length (Q))%nat ->
-  exists w', ixtransition w' = q /\ (length w' < length (Q))%nat /\
+  upper_bounded -> ixtransition w = q -> q <> (sink) ->
+  (length w >= length states)%nat ->
+  exists w', ixtransition w' = q /\ (length w' < length states)%nat /\
   count_buffer w' >= count_buffer w.
 Proof.
-  intro w.
-  revert q.
+  intro w; revert q;
   induction w as [|e w' IH] using @rev_ind; intros q H H0 H1 H2.
-  - assert (length (Q) > 0)%nat. {
-      pose proof (q0_correct). destruct (Q).
+  - assert (length states > 0)%nat. {
+      pose proof state0_correct. destruct states.
       destruct H3.
       simpl; omega.
     }
@@ -98,12 +120,11 @@ Proof.
       2: apply H0.
       2: auto.
       2: omega.
-      rewrite <- H4 in H.
-      apply H.
+      rewrite <- H4 in H; apply H.
     + unfold ixtransition in H0; rewrite ixtransition_distr in H0;
         fold ixtransition xtransition in H0.
-      pose H as H5.
-      eapply IH in H5. clear IH.
+      pose H as H5;
+      eapply IH in H5; clear IH.
       2: reflexivity.
       destruct H5 as [w0 [H6 [H7 H8]]].
       inversion H7.
@@ -130,21 +151,15 @@ Proof.
       -- rewrite app_length in H3; simpl in H3; omega.
 Qed.
 
+(* max_word q w is True if w counts the minimum items in q (maximum word) *)
 Definition max_word q w :=
   ixtransition w = q /\ forall w', ixtransition w' = q -> count_buffer w' <= count_buffer w.
 
-Lemma max_word_def q w :
-  (forall w', ixtransition w' = q -> count_buffer w' <= count_buffer w)
-  /\ ixtransition w = q <-> max_word q w.
-Proof.
-  split.
-  - intros [H H0]; unfold max_word; intuition.
-  - unfold max_word; intros [H H0]; intuition.
-Qed.
-
+(* a function that takes w1 and w2 and returns the sequence that counts most items *)
 Definition max w1 w2 :=
   if Z_ge_dec (count_buffer w1) (count_buffer w2) then w1 else w2.
 
+(* a function that returns the sequence of (possible) events of a given list that counts most items *)
 Fixpoint max_list (l:list (list B)) :=
   match l with
   | w::nil => w
@@ -152,7 +167,22 @@ Fixpoint max_list (l:list (list B)) :=
   | nil => nil
   end.
 
-Lemma max_list_correct1 l : forall q,
+(* Every sequence of (possible) events in l must count a number of items less or equal to count_buffer (max_list l). *)
+Lemma max_list_correct l : forall w,
+  In w l -> count_buffer w <= count_buffer (max_list l).
+Proof.
+  intros w H.
+  induction l as [|w' l' IH]; inversion H; simpl; unfold max.
+  - destruct (Z_ge_dec (count_buffer w') (count_buffer (max_list l'))) as [H1|H1].
+    + destruct l'; rewrite H0; intuition.
+    + apply Znot_ge_lt in H1; rewrite H0 in *; destruct l'; omega.
+  - apply IH in H0; destruct (Z_ge_dec (count_buffer w') (count_buffer (max_list l')));
+    destruct l'; try omega.
+    inversion H. rewrite H1; omega. destruct H1.
+Qed.
+
+(* If all the sequences of events in l transitions into q, max_list l does to. *)
+Lemma max_list_state l : forall q,
   l <> nil ->
   (forall w, In w l -> ixtransition w = q) ->
   ixtransition (max_list l) = q.
@@ -177,19 +207,7 @@ Proof.
       * apply H1.
 Qed.
 
-Lemma max_list_correct l : forall w,
-  In w l -> count_buffer w <= count_buffer (max_list l).
-Proof.
-  intros w H.
-  induction l as [|w' l' IH]; inversion H; simpl; unfold max.
-  - destruct (Z_ge_dec (count_buffer w') (count_buffer (max_list l'))) as [H1|H1].
-    + destruct l'; rewrite H0; intuition.
-    + apply Znot_ge_lt in H1; rewrite H0 in *; destruct l'; omega.
-  - apply IH in H0; destruct (Z_ge_dec (count_buffer w') (count_buffer (max_list l')));
-    destruct l'; try omega.
-    inversion H. rewrite H1; omega. destruct H1.
-Qed.
-
+(* a function that returns the [(possible) event] of a given list that adds most items *)
 Fixpoint max_in_list l :=
   match l with
   | e::nil => [e]
@@ -197,6 +215,7 @@ Fixpoint max_in_list l :=
   | nil => nil
   end.
 
+(* Every (possible) event in l must add a number of items less or equal to count_buffer (max_in_list l). *)
 Lemma max_in_list_correct l : forall e,
   In e l -> count_buffer [e] <= count_buffer (max_in_list l).
 Proof.
@@ -210,10 +229,12 @@ Proof.
     inversion H. rewrite H1; omega. destruct H1.
 Qed.
 
-Definition max_count_event := count_buffer (max_in_list (E)).
+(* count_buffer applied to the event that adds most items to the buffer *)
+Definition max_count_event := count_buffer (max_in_list events).
 
+(* Every event must add a number of items less or equal to max_count_event. *)
 Lemma max_count_event_correct : forall e,
-  In e (E) -> count_event e <= count_buffer (max_in_list (E)).
+  In e events -> count_event e <= max_count_event.
 Proof.
   intros e H.
   replace (count_event e) with (count_buffer [e]).
@@ -221,55 +242,44 @@ Proof.
   simpl; omega.
 Qed.
 
-Definition max_gen_words q := max_list (all_gen_words_le q (length (Q) - 1)).
+(* a function that returns the generated sequence of events w with length less than the number of states
+  such that w transitions into q and adds most items *)
+Definition max_gen_words q := max_list (all_gen_words_le q (length states - 1)).
 
+(* If the queueing system is upper bounded, every tangible state q is upper bounded. max_gen_words q must
+  count the maximum items in q. *)
 Lemma max_gen_words_correct q :
-  n_upper_bounded -> is_tangible q ->
+  upper_bounded -> is_tangible q ->
   max_word q (max_gen_words q).
 Proof.
   intros H H0.
-  apply max_word_def.
+  unfold max_word.
   split; unfold max_gen_words.
-  - intros w H1;
-    destruct H0 as [H0 H2];
-    destruct (le_gt_dec (length w) (length (Q) - 1)).
-    + apply max_list_correct, all_gen_words_le_correct; auto.
-    + assert (H3: (length w >= length (Q))%nat). omega.
-      eapply pumping_buffer with (q:=q) in H3.
-      2-4: auto.
-      destruct H3 as [w' [H3 [H4 H5]]].
-      assert (count_buffer w' <= count_buffer (max_list (all_gen_words_le q (length (Q) - 1)))).
-        apply max_list_correct, all_gen_words_le_correct; auto; omega.
-      omega.
-  - apply max_list_correct1.
-    + apply pumping in H0; destruct H0 as [w [H0 [H1 H2]]]; fold ixtransition in H0.
-      eapply all_gen_words_le_correct with (n:=(length (Q) - 1)%nat) in H2.
+  - apply max_list_state.
+    + apply tangible_length in H0; destruct H0 as [w [H0 [H1 H2]]]; fold ixtransition in H0.
+      eapply all_gen_words_le_generated with (n:=(length states - 1)%nat) in H2.
       2: apply H0.
       2: omega.
       intro contra; rewrite contra in H2; destruct H2.
     + intros w H1; unfold all_gen_words_le in H1;
-      eapply gen_words_correct1. 2: apply H1.
-      clear. induction (length (Q) - 1)%nat as [|n1 IH].
-      * simpl; intro contra; discriminate.
-      * simpl; destruct (all_words (S n1)) as [|a l]; auto.
-        simpl; intro contra; discriminate.
+      eapply gen_words_correct. apply H1.
+  - intros w H1;
+    destruct H0 as [H0 H2];
+    destruct (le_gt_dec (length w) (length states - 1)).
+    + apply max_list_correct, all_gen_words_le_generated; auto.
+    + assert (H3: (length w >= length states)%nat). omega.
+      eapply pumping_buffer with (q:=q) in H3.
+      2-4: auto.
+      destruct H3 as [w' [H3 [H4 H5]]].
+      assert (count_buffer w' <= count_buffer (max_list (all_gen_words_le q (length states - 1)))).
+        apply max_list_correct, all_gen_words_le_generated; auto; omega.
+      omega.
 Qed.
 
-Definition tangible_max_word q w := is_tangible q -> max_word q w.
-
-Lemma exists_max_word_function : n_upper_bounded ->
-    exists f, forall q, is_tangible q -> max_word q (f q).
-Proof.
-  intro H.
-  exists (max_gen_words);
-  intro q;
-  intro H0;
-  apply max_gen_words_correct; auto.
-Qed.
-
-Lemma max_word_q0 : forall w,
-  n_upper_bounded ->
-  max_word (q0) w ->
+(* The initial state's maximum word does not add items to the buffer if the queueing system is bounded. *)
+Lemma max_word_state0 : forall w,
+  upper_bounded ->
+  max_word state0 w ->
   count_buffer w = 0.
 Proof.
   intros w H H0.
@@ -277,17 +287,18 @@ Proof.
   destruct (count_buffer w) eqn:H1.
   - auto.
   - pose proof (Zgt_pos_0 p) as H2; rewrite <- H1 in H2, H3;
-    clear H1; pose H0 as H1; apply q0_cycle with (n:=2%nat) in H1;
+    clear H1; pose H0 as H1; apply state0_cycle with (n:=2%nat) in H1;
     apply H3 in H1. unfold count_buffer in H1; rewrite count_word_pow in H1; fold count_buffer in H1.
     nia.
   - pose proof (Zlt_neg_0 p) as H2; rewrite <- H1 in H2;
-    clear H0; assert (H0: ixtransition [] = q0). auto.
+    clear H0; assert (H0: ixtransition [] = state0). auto.
     apply H3 in H0; simpl in H0.
     omega.
 Qed.
 
+(* a lemma related to the second constraint of the function f *)
 Lemma max_word_transition : forall q e qe w we,
-  delta q e = qe -> qe <> sink ->
+  transition q e = qe -> qe <> sink ->
   max_word q w -> max_word qe we ->
   count_buffer we >= count_buffer w + count_event e.
 Proof.
@@ -300,48 +311,52 @@ Proof.
   omega.
 Qed.
 
+(* Now we prove that f exists and, for every tangible state q, f q must be less than max_items iff
+  the queueing system is correctly upper bounded. *)
 Theorem iff_exists_function__upper_bounded :
-  ( exists f, f (q0) >= (n0) /\ forall q, In q (Q) -> is_tangible q -> f q <= n /\
-    forall e, In e (E) -> f (delta q e) >= f q + count_event e )
-  <-> n_upper_bounded.
+  ( exists f, f state0 >= (init_items) /\ forall q, In q states -> is_tangible q -> f q <= max_items /\
+    forall e, In e events -> f (transition q e) >= f q + count_event e )
+  <-> upper_bounded.
 Proof.
   split.
 
-  - unfold n_upper_bounded; intros [ f [H H0] ] w H1.
-    cut (n0 + count_buffer w <= f (ixtransition w)).
-    cut (f (ixtransition w) <= n).
+  - unfold upper_bounded; intros [ f [H H0] ] w H1.
+    cut (init_items + count_buffer w <= f (ixtransition w)).
+    cut (f (ixtransition w) <= max_items).
     omega.
     apply H0.
-    apply ixtransition_in_Q; fold ixtransition; apply H1.
+    apply ixtransition_in_states; fold ixtransition; apply H1.
     split; try intuition; eexists; fold ixtransition; reflexivity.
     apply buffer_count_leq_f; try split; try (apply H0); intuition.
 
   - intro H.
-    pose H as H0; apply exists_max_word_function in H0; destruct H0 as [f H0];
-      unfold tangible_max_word in H0.
-    exists (fun q => if A_decidable q (sink) then (n)+(max_count_event) else (n0) + count_buffer (f q));
+    exists (fun q => if A_eq_dec q sink then (max_items)+(max_count_event) else (init_items) + count_buffer (max_gen_words q)).
     split.
-    + destruct (A_decidable (q0) (sink)) as [H2|H2].
-      destruct (sink_correct) as [_ contra]; symmetry in H2; contradiction.
-      assert (H1: is_tangible (q0)). split. auto. exists []; auto.
-      apply H0 in H1; apply max_word_q0 in H1; auto; omega.
-    + intros q H1 H2; pose H2 as H3; apply H0 in H3; destruct (A_decidable q (sink)).
-      destruct H2 as [H2 [w H4]]; contradiction.
-      assert (H4: n0 + count_buffer (f q) <= n). {
-        destruct H3 as [H3 _]; apply H; unfold is_generated;
-        fold ixtransition; destruct H2 as [H2 _]; rewrite <- H3 in H2; auto.
+    + destruct (A_eq_dec state0 sink) as [H2|H2].
+      destruct sink_correct as [_ [contra _]]; symmetry in H2; contradiction.
+      assert (H1: is_tangible state0). split. auto. exists []; auto.
+      apply max_word_state0 with (w:=max_gen_words state0) in H.
+      omega.
+      apply max_gen_words_correct; auto.
+    + intros q H0 H4; pose H4 as H1; destruct H1 as [H1 [w H2]].
+      destruct (A_eq_dec q sink) as [H3|_]. contradiction.
+      assert (H5: generates (max_gen_words q)). {
+          apply (max_gen_words_correct q) in H. 2: auto.
+          destruct H as [H _]; unfold generates; rewrite H; auto.
       }
       split.
-      * auto.
-      * intros e H5; destruct (A_decidable (delta q e) (sink)) as [H7|H7].
-        assert (count_event e <= max_count_event).
-          apply max_count_event_correct; auto.
+      * apply H; auto.
+      * intros e H3;
+        destruct (A_eq_dec (transition q e) sink).
+        apply max_count_event_correct in H3.
+        assert (init_items + count_buffer (max_gen_words q) <= max_items). auto.
         omega.
-        assert (H6: is_tangible (delta q e)).
-          split; auto; destruct H2 as [H2 [w H6]]; exists (w ++ [e]); rewrite ixtransition_distr;
-          simpl; rewrite H6; auto.
-        assert (count_buffer (f (delta q e)) >= count_buffer (f q) + count_event e).
-          eapply max_word_transition. 2: apply H7. reflexivity. apply H0; auto. apply H0; auto.
+        assert (count_buffer (max_gen_words (transition q e)) >= count_buffer (max_gen_words q) + count_event e). {
+          apply max_word_transition with (q:=q)(qe:=transition q e); auto.
+          1,2: apply max_gen_words_correct; auto.
+          split. auto.
+          exists (w ++ [e]); rewrite ixtransition_distr, H2; auto.
+        }
         omega.
 Qed.
 
