Utils.v
@@ -1,0 +1,15 @@
+Require Import Coq.Lists.List.
+Import ListNotations.
+
+(* If a list is not empty, the default value passed to function last
+  will not matter. *)
+Lemma last_any_default : forall {X} (l : list X) (a b : X),
+  l <> nil ->
+  last l a = last l b.
+Proof.
+  intros X l a b H; induction l as [|x l IH].
+  - contradiction.
+  - destruct l.
+    + auto.
+    + simpl in *; apply IH; intro contra; discriminate.
+Qed.
